

(3):

(a): Let  $X_n$  = number of type-a individuals at generation  $n$ .  
if  $X_n = i$ :

$$P(\text{type a individual is chosen to reproduce}) = \frac{i}{N}$$

$$\rightarrow P(\text{type A} \leftarrow) = \frac{N-i}{N}$$

$$\Rightarrow P(X_n = X_n + 1): p_{i,i+1} = \frac{i}{N} \cdot \frac{N-i}{N}$$

$\boxed{\text{chose a}}$ 
 $\boxed{\text{reproduce by a, chose A}}$

$$\Rightarrow P(X_n = X_n - 1): p_{i,i-1} = \frac{N-i}{N} \cdot \frac{i}{N} \quad (\text{opposite})$$

$$\Rightarrow P(X_n = X_n): p_{i,i} = \frac{i^2}{N^2} + \frac{(N-i)^2}{N^2}$$

$\boxed{\text{double chose a}}$ 
 $\boxed{\text{double chose A}}$

boundary state:

$$p_{0,0} = 1 = p_{N,N} \quad (\text{absorbing state})$$

(b): Let  $u(i) = P(\underbrace{\text{absorbed at } N}_{(A)}, \underbrace{\text{before hitting } 0}_{(a)})$

$$u(i) = p_{i,i-1}u(i-1) + p_{i,i}u(i) + p_{i,i+1}u(i+1)$$

$$\rightarrow p_{i,i+1}u(i+1) + (p_{i,i} - 1)u(i) + p_{i,i-1}u(i-1)$$

boundary:  $u(0) = 0, u(N) = 1$

(c): recurrence to eliminate  $u(i+1)$ , get:

$$p_{i,i+1} \cdot d(i) = p_{i,i-1} \cdot d(i-1)$$

$$\text{and: } p_{i,i+1} = p_{i,i-1} = \frac{i(N-i)}{N^2} \rightarrow d(i) = d(i-1) \Rightarrow d(i) \text{ is a constant.}$$

$$\rightarrow u(i) = u(0) + \sum_{k=0}^{i-1} d = i \cdot d \rightarrow \text{By condition } u(N) = 1: \rightarrow$$

$$d = \frac{1}{N} \Rightarrow u(i) = \frac{i}{N} \quad \text{for every step is } \pm 1$$

*Algebra*

(1):  $h_0^{\{0\}} = 0$  and  $h_N^{\{0\}} = \infty$ , we can get easily

For the other state  $1 \leq i \leq N-1$ :

$$\underline{h_i^{\{0\}}} = 1 + \frac{1}{2} \underline{h_{i+1}^{\{0\}}} + \frac{1}{2} \underline{h_{i-1}^{\{0\}}}$$

we set a quadratic form:

$$\begin{aligned} \underline{A + Bi + Ci^2} &= 1 + \frac{1}{2} (h_{i+1}^{\{0\}} + h_{i-1}^{\{0\}}) \\ &= 1 + \frac{1}{2} (2A + B(i+1 + i-1) + C(i^2 + 2i + 1 + i^2 - 2i + 1)) \\ &= 1 + \frac{1}{2} (2A + 2Bi + 2Ci^2 + 2C) \\ &= 1 + \underline{A + Bi + Ci^2} + C \end{aligned}$$

$$\Rightarrow 0 = 1 + C \rightarrow C = -1$$

$$h_i^{\{0\}} = A + Bi - i^2$$

when  $i = 0$ :

$$0 = A \rightarrow A = 0$$

$\rightarrow h_i^{\{0\}} = i(B - i) \rightarrow$  if  $B = N$ , expected hitting time to either.

But we only consider one edge, so  $h_i^{\{0\}} = i(2N - i) \quad (0 \leq i \leq \infty)$

(2): let  $p_{i,i-1} = q_i$

$$\Rightarrow p_{i,i+1} = \left(\frac{i+1}{i}\right)^\beta q_i \rightarrow q_i + \left(\frac{i+1}{i}\right)^\beta q_i = 1 \rightarrow q_i = \frac{1}{1 + \left(\frac{i+1}{i}\right)^\beta}$$

consider  $i$ :

$$\text{when } i \rightarrow \infty: \frac{i+1}{i} \sim 1 + \frac{1}{i} \Rightarrow \left(\frac{i+1}{i}\right)^\beta \sim 1 + \frac{\beta}{i}$$

$$q_i \rightarrow \frac{1}{1 + 1 + \frac{\beta}{i}} = \frac{1}{2 + \frac{\beta}{i}} \sim \frac{1}{2} - \frac{\beta}{4i} \rightarrow \begin{cases} \beta > 0, \text{ far away} \\ \beta < 0, \text{ closer} \end{cases}$$

$$\sum_{i=1}^{\infty} \left(\frac{i+1}{i}\right)^\beta = \lim_{n \rightarrow \infty} (n+1)^\beta \rightarrow \beta \text{ needs: } \beta < 0 \text{ to } \text{closed touch} \text{ to } 0$$